secure_api/merkle_tree/MerkleTree.fsti
@@ -251,6 +251,3 @@ let mt_deserialize_path
   (len:UInt64.t{CB.length buf = U64.v len})
 : HST.ST (B.pointer_or_null (path #hash_size)) pf pt
 = MTNLS.mt_deserialize_path #hash_size rid buf len
-
-[@ (Comment "  Default hash function")]
-let mt_sha256_compress: MTNLHF.hash_fun_t #32ul #(Ghost.hide MTS.sha256_compress) = MTNLE.sha256_compress
